decrypt'

src/QUIC.Impl.fst
@@ -1065,15 +1065,15 @@ let payload_decrypt_pre
   (s: AEAD.state a)
   (siv: B.buffer Secret.uint8)
   (dst: B.buffer Secret.uint8)
-  (h: header { ~ (is_retry h) })
-  (pn: Ghost.erased (PN.packet_number_t))
+  (gh: Ghost.erased Spec.header { ~ (Spec.is_retry gh) })
+  (hlen: Secret.uint32)
+  (pn_len: PN.packet_number_length_t)
+  (pn: PN.packet_number_t)
   (cipher_and_tag_len: Secret.uint32)
   (m: HS.mem)
 : GTot Type0
 =
-  let gh = g_header h m pn in
   let fmt = SParse.format_header gh in
-  let hlen = header_len h in
 
   B.all_disjoint [
     AEAD.footprint m s;
@@ -1084,9 +1084,12 @@ let payload_decrypt_pre
   AEAD.invariant m s /\
   B.live m siv /\ B.length siv == 12 /\
   Secret.v cipher_and_tag_len >= SAEAD.tag_length a /\
+  Secret.v hlen == Seq.length fmt /\
   Secret.v hlen + Secret.v cipher_and_tag_len <= B.length dst /\
   Secret.v cipher_and_tag_len < max_cipher_length /\
   B.live m dst /\
+  pn_len == Spec.pn_length gh /\
+  pn == Spec.packet_number gh /\
   B.as_seq m (B.gsub dst 0ul (Secret.reveal hlen)) `Seq.equal` Seq.seq_hide fmt
 
 unfold
@@ -1095,24 +1098,26 @@ let payload_decrypt_post
   (s: AEAD.state a)
   (siv: B.buffer Secret.uint8)
   (dst: B.buffer Secret.uint8)
-  (h: header { ~ (is_retry h) })
-  (pn: G.erased PN.packet_number_t)
+  (gh: Ghost.erased Spec.header { ~ (Spec.is_retry gh) })
+  (hlen: Secret.uint32)
+  (pn_len: PN.packet_number_length_t)
+  (pn: PN.packet_number_t)
   (cipher_and_tag_len: Secret.uint32)
   (m: HS.mem)
   (res: error_code)
   (m' : HS.mem)
 : GTot Type0
 =
-  payload_decrypt_pre a s siv dst h pn cipher_and_tag_len m /\
+  payload_decrypt_pre a s siv dst gh hlen pn_len pn cipher_and_tag_len m /\
   begin
-    let bplain = B.gsub dst (Secret.reveal (header_len h)) (Secret.reveal cipher_and_tag_len `U32.sub` U32.uint_to_t (SAEAD.tag_length a)) in
+    let bplain = B.gsub dst (Secret.reveal hlen) (Secret.reveal cipher_and_tag_len `U32.sub` U32.uint_to_t (SAEAD.tag_length a)) in
     B.modifies (B.loc_buffer bplain `B.loc_union` AEAD.footprint m s) m m' /\
     AEAD.invariant m' s /\ AEAD.footprint m' s == AEAD.footprint m s /\
     AEAD.preserves_freeable s m m' /\
     AEAD.as_kv (B.deref m' s) == AEAD.as_kv (B.deref m s) /\
-    begin match res, Spec.payload_decrypt a (AEAD.as_kv (B.deref m s)) (B.as_seq m siv) (g_header h m pn) (B.as_seq m (B.gsub dst (Secret.reveal (header_len h)) (Secret.reveal cipher_and_tag_len))) with
+    begin match res, Spec.payload_decrypt a (AEAD.as_kv (B.deref m s)) (B.as_seq m siv) gh (B.as_seq m (B.gsub dst (Secret.reveal hlen) (Secret.reveal cipher_and_tag_len))) with
     | Success, Some plain ->
-True //      B.as_seq m' bplain `Seq.equal` plain
+      B.as_seq m' bplain `Seq.equal` plain
     | AuthenticationFailure, None -> True
     | _ -> False
     end
@@ -1125,22 +1130,20 @@ let payload_decrypt
   (s: AEAD.state a)
   (siv: B.buffer Secret.uint8)
   (dst: B.buffer Secret.uint8)
-  (h: header { ~ (is_retry h) })
+  (gh: Ghost.erased Spec.header { ~ (Spec.is_retry gh) })
+  (hlen: Secret.uint32)
+  (pn_len: PN.packet_number_length_t)
   (pn: PN.packet_number_t)
   (cipher_and_tag_len: Secret.uint32)
 : HST.Stack error_code
   (requires (fun m ->
-    payload_decrypt_pre a s siv dst h pn cipher_and_tag_len m
+    payload_decrypt_pre a s siv dst gh hlen pn_len pn cipher_and_tag_len m
   ))
   (ensures (fun m res m' ->
-    payload_decrypt_post a s siv dst h pn cipher_and_tag_len m res m'
+    payload_decrypt_post a s siv dst gh hlen pn_len pn cipher_and_tag_len m res m'
   ))
 = 
   let m0 = HST.get () in
-  let hlen = header_len h in
-  QUIC.Impl.Header.Parse.header_len_correct h m0 pn;
-  let pn_len = pn_length h in
-  let gh = Ghost.hide (g_header h m0 pn) in
   HST.push_frame ();
   let m1 = HST.get () in
   B.loc_unused_in_not_unused_in_disjoint m1;
@@ -1229,17 +1232,21 @@ let decrypt'_post
     header_live h m' /\
     r.header_len == header_len h /\
     Secret.v r.plain_len == Seq.length plain /\
-    Secret.v r.header_len + Secret.v r.plain_len == Secret.v r.total_len /\
+    Secret.v r.header_len + Secret.v r.plain_len <= Secret.v r.total_len /\
     Secret.v r.total_len <= B.length dst /\ (
       let dst_mod = B.gsub dst 0ul (Secret.reveal r.total_len) in
       B.modifies (AEAD.footprint m aead `B.loc_union` CTR.footprint m ctr `B.loc_union` B.loc_buffer dst_hdr `B.loc_union` B.loc_buffer dst_mod) m m' /\
-      B.as_seq m' dst `Seq.equal` (QUIC.Spec.Header.Parse.format_header (g_header h m' r.pn) `Seq.append` plain `Seq.append` rem)
+      B.as_seq m' (B.gsub dst 0ul (Secret.reveal r.header_len)) `Seq.equal` QUIC.Spec.Header.Parse.format_header (g_header h m' r.pn) /\
+      B.as_seq m' (B.gsub dst (Secret.reveal r.header_len) (Secret.reveal r.plain_len)) `Seq.equal` plain /\
+      B.as_seq m' (B.gsub dst (Secret.reveal r.total_len) (B.len dst `U32.sub` Secret.reveal r.total_len)) `Seq.equal` rem
     )
-  | _ -> False
+  | _ -> True
   end
 
-(*
-#push-options "--z3rlimit 64"
+#push-options "--z3rlimit 256"
+
+#restart-solver
+
 let decrypt'
   (a: ea)
   (aead: AEAD.state a)
@@ -1262,6 +1269,12 @@ let decrypt'
   match QUIC.Impl.Header.header_decrypt a ctr hpk cid_len last_pn dst dst_len with
   | QUIC.Impl.Header.H_Failure -> DecodeError
   | QUIC.Impl.Header.H_Success h pn cipher_and_tag_len ->
+    assert (
+      match QUIC.Spec.Header.header_decrypt a (B.as_seq m0 hpk) (U32.v cid_len) (Secret.v last_pn) (B.as_seq m0 dst) with
+      | QUIC.Spec.Header.H_Success _ ct _ ->
+        Seq.length ct == Secret.v cipher_and_tag_len
+      | _ -> False
+    );
     let m1 = HST.get () in
     let hlen = header_len h in
     QUIC.Impl.Header.Parse.header_len_correct h m1 pn;
@@ -1279,52 +1292,63 @@ let decrypt'
       QUIC.Impl.Header.Base.frame_header h pn (B.loc_buffer dst_hdr) m1 m2;
       Success
     end else begin
-      let res = SecretBuffer.with_whole_buffer_hide_weak_modifies
+      let gh : Ghost.erased Spec.header = Ghost.hide (g_header h m1 pn) in
+      let pn_len = pn_length h in
+      B.gsub_zero_length dst;
+      assert (Secret.v cipher_and_tag_len >= 16);
+      assert (SAEAD.tag_length a == 16);
+      let plain_len = cipher_and_tag_len `Secret.sub` Secret.hide 16ul in
+      let res = SecretBuffer.with_buffer_hide_from
         #error_code
         dst
+        0ul
         m1
-        (AEAD.footprint m0 aead `B.loc_union`
+        (AEAD.footprint m1 aead `B.loc_union`
           B.loc_buffer siv `B.loc_union`
-          CTR.footprint m0 ctr `B.loc_union`
-          B.loc_buffer hpk `B.loc_union`
-          B.loc_buffer dst_hdr)
-        (AEAD.footprint m0 aead)
-        true
-        (fun res cont m_ ->
-          res == Success /\
-          cont `Seq.equal` (
-            fmt `Seq.append`
-            Spec.payload_encrypt a (AEAD.as_kv (B.deref m0 aead)) (B.as_seq m0 siv) (g_header h m0 pn) (Seq.seq_reveal (B.as_seq m0 plain))) /\
+          CTR.footprint m1 ctr `B.loc_union`
+          B.loc_buffer hpk)
+        (AEAD.footprint m1 aead)
+        1ul 0ul (Secret.reveal hlen) (Secret.reveal hlen `U32.add` (Secret.reveal cipher_and_tag_len `U32.sub` U32.uint_to_t (SAEAD.tag_length a)))
+        (fun res _ cont m_ ->
+          begin match res, Spec.payload_decrypt a (AEAD.as_kv (B.deref m1 aead)) (B.as_seq m1 siv) gh (Seq.seq_hide (B.as_seq m1 (B.gsub dst (Secret.reveal hlen) (Secret.reveal cipher_and_tag_len)))) with
+          | Success, Some plain ->
+            Seq.slice cont (Secret.v hlen) (Secret.v hlen + (Secret.v cipher_and_tag_len - SAEAD.tag_length a)) == Seq.seq_reveal plain
+          | AuthenticationFailure, None -> True
+          | _ -> False
+          end /\
           AEAD.invariant m_ aead /\ AEAD.footprint m_ aead == AEAD.footprint m0 aead /\
           AEAD.preserves_freeable aead m1 m_ /\
           AEAD.as_kv (B.deref m_ aead) == AEAD.as_kv (B.deref m0 aead)
         )
-        (fun _ bs -> 
-          let res = payload_encrypt a aead siv bs gh pn_len pn header_len plain plain_len in
+        (fun _ _ bs ->
+          let res = payload_decrypt a aead siv bs gh hlen pn_len pn cipher_and_tag_len in
           let m_ = HST.get () in
           assert (
-            let cont = B.as_seq m_ bs in
-            Seq.length fmt == Secret.v header_len /\
-            cont `Seq.equal` (Seq.slice cont 0 (Secret.v header_len) `Seq.append` Seq.slice cont (Secret.v header_len) (Seq.length cont))
+            let cont = Seq.seq_reveal (B.as_seq m_ bs) in
+            match res, Spec.payload_decrypt a (AEAD.as_kv (B.deref m1 aead)) (B.as_seq m1 siv) gh (Seq.seq_hide (B.as_seq m1 (B.gsub dst (Secret.reveal hlen) (Secret.reveal cipher_and_tag_len)))) with
+            | Success, Some plain ->
+            Seq.slice cont (Secret.v hlen) (Secret.v hlen + (Secret.v cipher_and_tag_len - SAEAD.tag_length a)) `Seq.equal` Seq.seq_reveal plain
+            | AuthenticationFailure, None -> True
+            | _ -> False
           );
           res
         )
       in
-
-  
-      let res = payload_decrypt a aead siv dst h pn cipher_and_tag_len in
-      let plain_len = cipher_and_tag_len `Secret.sub` Secret.hide 16ul in
       let r = {
         pn = pn;
         header = h;
         header_len = hlen;
         plain_len = plain_len;
-        total_len = hlen `Secret.add` plain_len;
+        total_len = hlen `Secret.add` cipher_and_tag_len;
       } in
       B.upd dst_hdr 0ul r;
+      let m3 = HST.get () in
+      QUIC.Impl.Header.Base.frame_header h pn
+        (AEAD.footprint m1 aead `B.loc_union` CTR.footprint m1 ctr `B.loc_union` B.loc_buffer dst_hdr `B.loc_union` B.loc_buffer (B.gsub dst (Secret.reveal hlen) (B.len dst `U32.sub` Secret.reveal hlen))) m1 m3;
       res
     end
-*)    
+
+#pop-options
 
 
 let decrypt
